basic_nonlifted

theories/SLFBasicLifted.v
@@ -10,11 +10,14 @@ License: MIT.
 *)
 
 Set Implicit Arguments.
-From Sep Require Import SLFDirect SLFExtra.
-Import SLFProgramSyntax DemoPrograms ExtraDemoPrograms.
+From Sep Require Import Example.
+Generalizable Variables A B.
 
 Implicit Types n m : int.
 Implicit Types p q : loc.
+
+(** Tweak to make the logic appear linear instead of affine. *)
+Ltac xwp_xtriple_handle_gc ::= xwp_xtriple_remove_gc.
 
 
 (* ########################################################### *)
@@ -23,24 +26,26 @@ Implicit Types p q : loc.
 (** * Chapter in a rush, nested with exercises as additional contents *)
 
 (** This chapter gives a quick overview of how to state specifications and
-    carry out basic proofs in Separation Logic using the framework whose
-    construction is presented throughout this course.
+    carry out basic proofs in Separation Logic using CFML tactics.
 
     In this chapter, we will present:
 
     - "Heap predicates", which are used to describe memory states in
-      Separation Logic.
-    - "Specification triples", of the form [triple t H Q].
+       Separation Logic.
+    - "Specification triples", of the form [TRIPLE _ PRE _ POST _].
       Such specification relate a term, a precondition, and a postcondition.
+    - "Verification proof obligations", of the form [PRE _ CODE _ POST _].
+      These proof obligations also correspond to specification triples, yet
+      they feature the description of the current state as first argument
+      in order to improve readability of proof obligations.
     - "Entailment proof obligations", of the form [_ ==> _] or [_ ===> _].
       Such entailments require proving that a description of a state implies
       another one.
-    - "Verification proof obligations", of the form [PRE H CODE F POST Q].
-    - Verification tactics, called "x-tactics", which are specialized tactics
-      for carrying out the verification proofs.
+    - Practical verification proofs, using CFML "x-tactics" to demonstrate
+      that a given program satisfies a given specification.
 
     The "heap predicates" used to describe memory states include:
-    - [p ~~~> n], which describes a memory cell at location [p] with contents [n],
+    - [p ~~> n], which describes a memory cell at location [p] with contents [n],
     - [\[]], which describes an empty state,
     - [\[P]], which asserts that a proposition [P] is true (in an empty state),
     - [H1 \* H2], which describes a state made of two disjoint parts: [H1] and [H2],
@@ -49,10 +54,10 @@ Implicit Types p q : loc.
     All these heap predicates admit the type [hprop], which consists of predicate
     over memory states. In other words, [hprop] is defined as [state->Prop].
 
-    The verification proofs are carried out using x-tactics, identified by the
-    leading "x" letter in their name. These tactics include:
-    - [xwp] or [xtriple] to being a proof,
-    - [xapp] to reason about an application,
+    The verification proofs are carried out using CFML "x-tactics", as their
+    name begins with the letter "x". These tactics include:
+    - [xwp] or [xtriple] to being a proof (in case of failure, try [xwp_debug]),
+    - [xapp] to reason about an application (in case of failure, try [xapp_debug]),
     - [xval] to reason about a return value,
     - [xsimpl] to simplify or prove entailments ([_ ==> _] or [_ ===> _]). *)
 
@@ -64,11 +69,6 @@ Implicit Types p q : loc.
     - [gen], which is a shorthand for [generalize dependent], a tactic
       also useful to set up induction principles.
 
-   For simplicity, we assume all programs to be written in A-normal form,
-   that is, with all intermediate expressions being named by a let-binding.
-   Every example program is first informally presented in OCaml syntax, then
-   is formally defined in Coq using an ad-hoc notation system, featuring
-   variable names and operators all prefixed by a quote symbol.
 *)
 
 
@@ -80,24 +80,24 @@ Implicit Types p q : loc.
     In OCaml syntax, this function is defined as:
 
 [[
-   let incr p =
-       let n = !p in
-       let m = n + 1 in
-       p := m
+    let incr p =
+      p := !p + 1
 ]]
 
-    We input this program using a custom set of Coq notation for describing
-    imperative programs. There is no need to learn how to write programs in
-    this funny syntax: the source code for all the programs involved in this
-    course is provided.
+    The actual CFML tool features a parser able to process OCaml syntax.
+    Yet, throughout this course, to avoid dependency on an external tool,
+    we will input all programs using a custom set of Coq notation for
+    describing imperative programs. There is no need to learn how to write
+    programs in this funny syntax: the source code for all the programs
+    involved in this course is provided.
 
-    Below is the definition for the function [incr]. This function is a value,
+    Below is the code for the function [incr]. This function is a value,
     so it admits, like all values in the CFML framework, the type [val].
 
     The quotes that appear in the source code are used to disambiguate
     between the keywords and variables associated with the source code,
     and those from the corresponding Coq keywords and variables.
-    The [VFun] keyword should be read like the [fun] keyword from OCaml.
+    The [VFun] keyword should be read like the [fun] keyword.
 
     Again, the details of this funny syntax are not important, the reader
     may blindly trust that it corresponds to the OCaml code shown above.
@@ -105,107 +105,124 @@ Implicit Types p q : loc.
 
 Definition incr : val :=
   VFun 'p :=
-    Let 'n := '! 'p in
-    Let 'm := 'n '+ 1 in
-    'p ':= 'm.
+   'p ':= '! 'p '+ 1.
 
-(** The specification of [incr p], shown below, is expressed using a
-    "Separation Logic triple". A triple is formally expressed by a proposition
-    of the form [triple t H Q]. By convention, we write the precondition [H]
-    and the postcondition [Q] on separate lines. Details are explained next. *)
-
-Lemma triple_incr : forall (p:loc) (n:int),
-  triple (incr p)
-    (p ~~~> n)
-    (fun _ => (p ~~~> (n+1))).
-
-(** Above, [p] denotes the address in memory of the reference cell provided
-    as argument to the increment function. In technical vocabulary, [p]
-    is the "location" of a reference cell. All locations have type
+(** Let [p] be the address in memory of the reference cell provided as
+    argument to the increment function. In technical vocabulary, [p]
+    is the "location" of a reference cell. In CFML, locations have type
     [loc], thus the argument [p] of [incr] has type [loc].
 
-    In Separation Logic, the "heap predicate" [p ~~~> n] describes a memory
+    In Separation Logic, the "heap predicate" [p ~~> n] describes a memory
     state in which the contents of the location [p] is the value [n].
     In the present example, [n] denotes an integer value.
 
     The behavior of the operation [incr p] consists of updating the memory
     state by incrementing the contents of the cell at location [p], so that
     its new contents is [n+1]. Thus, the memory state posterior to the
-    increment operation can be described by the heap predicate [p ~~~> (n+1)].
+    increment operation can be described by the heap predicate [p ~~> (n+1)].
 
-    The result value returned by [incr p] is the unit value, which does not
-    carry any useful information. In the specification of [incr], the
-    postcondition is of the form [fun _ => ...] to indicate that there is
-    no need to bind a name for the result value. *)
+    The result value returned by [incr p] is the [unit] value. There is not
+    much to specify about the result value, beyond the fact that it has
+    type [unit]. In the specification of [incr], the notation
+    [fun (r:unit) => ...] indicates that the result has type [unit].
 
-(** The general pattern of a specification thus includes:
+    The specification of [incr p], shown below, is expressed using a
+    "Separation Logic triple", stated using the custom notation
+    [TRIPLE _ PRE _ POST _], whose compontents are explained next. *)
 
-    - Quantification of the arguments (here [p]) and of the "ghost variables"
-      (here, [n]) used to describe the input state.
-    - The application of the predicate [triple] to the function application
-      [incr p], which is the term being specified by the triple.
-    - The precondition describing the input state, here [p ~~~> n].
-    - The postcondition describing both the output value and the output state.
-      The general pattern is [fun r => H'], where [r] denotes the name of
-      the result, and [H'] describes the final state. Here, the final
-      state is described by [p ~~~> (n+1)]. *)
+Lemma Triple_incr : forall (p:loc) (n:int),
+  TRIPLE (incr p)
+    PRE (p ~~> n)
+    POST (fun (r:unit) => (p ~~> (n+1))).
 
-(** Remark: we have to write [p ~~~> (n+1)] using parentheses around [n+1],
-    because [p ~~~> n+1] would get parsed as [(p ~~~> n) + 1]. *)
+(** The components form this specification are as follows:
 
-(** Our next step is to prove the specification lemma [triple_incr] which
+    - [forall (p:loc) (n:int)] quantifies the argument of the function
+      (here, [p]), as well as the "ghost argument" (here, [n]) which is used
+      to describe the input state.
+    - The keyword [TRIPLE] introduces the expression [incr p], which is the
+      function being specified.
+    - The keyword [PRE] introduces the "precondition", which describes the
+      input state that the function expects, here [p ~~> n].
+    - The keyword [POST] introduces the "postcondition", which describes
+      both the output value and the output state produced by the call.
+      The pattern [fun (r:unit) => _] binds the name [r] to denote the result
+      value; here [r] has type unit, reflecting the type of [incr p].
+      Finally, the expression [p ~~> (n+1)] describes the output state. *)
+
+(** Remark: we have to write [p ~~> (n+1)] using parentheses around [n+1],
+    because [p ~~> n+1] would get parsed as [(p ~~> n) + 1]. *)
+
+(** Our next step is to prove the specification lemma [Triple_incr] which
     specifies the behavior of the function [incr]. We conduct the
-    verification proof using x-tactics. *)
+    verification proof using CFML tactics.
+
+    The CFML tooling will transform on-the-fly the code so that all
+    intermediate expressions are named, that is, by putting the code
+    in "A-normal form". In OCaml syntax, the A-normal could be written:
+
+[[
+    let incr p =
+      let m =
+        let n = !p in
+        n + 1 in
+      p := m
+]]
+
+    The transformation into A-normal form is performed by the tactic [xwp],
+    which begins every CFML verification proof script. The tactic [xwp]
+    also sets up the goal in the form that is ready for verification using
+    CFML "x-tactics". What happens behind the scene is explained much later
+    in the chapter [SLFWPgen]. For now, we focus on the high-level aspect
+    of the proofs, from an end-user point of view.
+*)
 
 Proof using.
   xwp.     (* Begin the verification proof. The proof obligation is
-              displayed using the custom notation [PRE H CODE F POST Q].
+              displayed using the custom notation [PRE _ CODE _ POST _].
               The [CODE] part does not look very nice, but one should
               be able to somehow recognize the body of [incr]. Indeed,
-              if we ignoring the details, and perform the alpha-renaming
-              from [v] to [n] and [v0] to [m], the [CODE] section reads like:
+              if we ignoring the details, and perform the relevant
+              alpha-renaming, the [CODE] section reads like:
 [[
-              Let' n := (App val_get p) in
-              Let' m := (App val_add n 1) in
-              App val_set p m
+              Let m :=
+                  Let n := App val_get p in
+                  App val_add n 1
+                  in
+               App val_set p m
 ]]
-              which is somewhat similar to the original source code.
-           *)
+              which is similar to the OCaml syntax in A-normal form.
+   *)
 
  (*  The remaining of the proof performs some form of symbolic
      execution. One should not attempt to read the full proof
      obligation at each step, but instead only look at the current
-     state, described by the [PRE] part (here, [p ~~~> n]), and at
+     state, described by the [PRE] part (here, [p ~~> n]), and at
      the first line only of the [CODE] part, where one can read
      the code of the next operation to reason about.
 
      Each function call is handled using the tactic [xapp]. *)
 
-  xapp.    (* Reason about the operation [!p] that reads into [p];
+  xapp.    (* Reason about the the operation [!p] that reads into [p];
               the read operation returns the value [n]. *)
   xapp.    (* Reason about the addition operation [n+1]. *)
   xapp.    (* Reason about the update operation [p := n+1],
-              thereby updating the state to [p ~~~> (n+1)]. *)
+              thereby updating the state to [p ~~> (n+1)]. *)
   xsimpl.  (* At this stage, the proof obligation takes the form [_ ==> _],
               which require checking that the final state matches what
               is claimed in the postcondition. [xsimpl] takes care of it. *)
 Qed.
 
-(** The command below associates the specification lemma [triple_incr]
+(** The command below associates the specification lemma [Triple_incr]
     with the function [incr] in a database, so that if we subsequently
     verify a program that features a call to [incr], the [xapp] tactic
-    is able to automatically invoke the lemma [triple_incr]. *)
+    is able to automatically invoke the lemma [Triple_incr]. *)
 
-Hint Resolve triple_incr : triple.
+Hint Extern 1 (Register_Spec incr) => Provide Triple_incr.
 
-(** Remark: the proof framework can be used without any knowledge about
-    the implementation of the notation [PRE H CODE F POST Q] nor about
-    the implementation of the x-tactics.
-
-    A reader with prior knowledge in program verification might
-    nevertheless be interested to know that [PRE H CODE F POST Q]
-    is defined as the [H ==> F Q], where [F] is a form of weakest-
-    precondition that describes the behavior of the code. *)
+(** Remark: there is no need to understand the internal magic of how
+    this database of specification is implemented by hacking Coq's
+    [Hint] mechanism. *)
 
 
 (* ########################################################### *)
@@ -232,25 +249,22 @@ Definition example_let : val :=
     'a '+ 'b.
 
 (** We specify this function using the the triple notation, in the form
-    [triple (example_let n) H (fun r => H')], where [r], of type [val],
-    denotes the output value.
+    [TRIPLE (example_let n) PRE _ POST (fun (r:int) => _ )], where [r]
+    denotes the output value. This time, the output value has type [int].
 
     To denote the fact that the input state is empty, we write [\[]]
-    in the precondition.
+    in the precondition, that is, after the [PRE] keyword.
 
     To denote the fact that the output state is empty, we could use [\[]].
-    Yet, if we writ just [fun r => \[]] as postcondition, we would have
+    Yet, if we write [fun (r:int) => \[]] as postcondition, we would have
     said nothing about the output value [r] produced by a call [example_let].
     Instead, we would like to specify that the result [r] is equal to [2*n].
-    To that end, we write the postcondition [fun r => \[r = 2*n]], which
-    actually stands for [fun (r:val) => [r = val_int (2*n)], where the
-    coercion [val_int] translates the integer value [2*n] into the
-    corresponding value of type [val] from the programming language. *)
+    To that end, we write [fun (r:int) => \[r = 2*n]] after the [POST] keyword. *)
 
-Lemma triple_example_let : forall (n:int),
-  triple (example_let n)
-    \[]
-    (fun r => \[r = 2*n]).
+Lemma Triple_example_let : forall (n:int),
+  TRIPLE (example_let n)
+    PRE \[]
+    POST (fun (r:int) => \[r = 2*n]).
 
 (** The verification proof script is very similar to the previous one.
     The x-tactics [xapp] performs symbolic execution of the code.
@@ -262,12 +276,39 @@ Proof using.
   xwp. xapp. xapp. xapp. xsimpl. math.
 Qed.
 
+(** In the proof above, we have eagerly substituted [a] with [n+1],
+    then substituted [b] with [n-1]. Such eager substitutions generally
+    work well for small programs, yet in larger programs doing so can lead
+    to exponential blow-ups in the size of the terms being manipulated.
+    To avoid such blow-ups, it may be necessary to preserve explicit
+    equalities, such as [a = n+1] and [b = n-1], in the proof context.
+
+    In general, it is desirable to let the user control when substitutions
+    should or should not be performed. Where the [xapp] tactic systematically
+    attempts to perform a substitution, its variant [xapp_nosubst] instead
+    introduces an explicit equality, as illustrated next. *)
+
+Lemma Triple_example_let_with_nosubst : forall (n:int),
+  TRIPLE (example_let n)
+    PRE \[]
+    POST (fun (r:int) => \[r = 2*n]).
+Proof using.
+  xwp.
+  xapp_nosubst. intros a Ha.  (* introduces [Ha: a = n + 1] *)
+  xapp_nosubst. intros b Hb.  (* introduces [Hb: b = n - 1] *)
+  xapp_nosubst. intros r Hr.  (* introduces [Hb: r = a + b] *)
+  xsimpl. math. (* check that, under these hypotheses, [r = 2 * n]. *)
+Qed.
+
+(** Throughout the course, we only consider programs that are simple
+    enough that one may use the tactic [xapp] everywhere. *)
+
 
 (* ########################################################### *)
 (** ** Exercise: function [quadruple] *)
 
 (** Consider the function [quadruple], which expects an integer [n]
-    and returns its quadruple, that is, the value [4*n].
+    and returns its quadruple, that is, the value [4 * n].
 
 [[
     let quadruple n =
@@ -280,16 +321,16 @@ Definition quadruple : val :=
     Let 'm := 'n '+ 'n in
     'm '+ 'm.
 
-(* EX1! (triple_quadruple) *)
+(* EX1! (Triple_quadruple) *)
 (** Specify and verify the function [quadruple] to express that
     it returns [4*n].
-    Hint: follow the template of [triple_example_let]. *)
+    Hint: follow the template of [Triple_example_let]. *)
 
 (* SOLUTION *)
-Lemma triple_quadruple : forall (n:int),
-  triple (quadruple n)
-    \[]
-    (fun r => \[r = 4 * n]).
+Lemma Triple_quadruple : forall (n:int),
+  TRIPLE (quadruple n)
+    PRE \[]
+    POST (fun (r:int) => \[r = 4 * n]).
 Proof using.
   xwp. xapp. xapp. xsimpl. math.
 Qed.
@@ -307,29 +348,25 @@ Qed.
 
 [[
     let inplace_double p =
-      let n = !p in
-      let m = n + n in
-      p := m
+      p := !p + !p
 ]]
 *)
 
 Definition inplace_double : val :=
   VFun 'p :=
-    Let 'n := '!'p in
-    Let 'm := 'n '+ 'n in
-    'p ':= 'm.
+    'p ':= ('!'p '+ '!'p).
 
-(* EX1! (triple_inplace_double) *)
+(* EX1! (Triple_inplace_double) *)
 (** Specify and verify the function [inplace_double].
-    Hint: follow the template of [triple_incr]. *)
+    Hint: follow the template of [Triple_incr]. *)
 
 (* SOLUTION *)
-Lemma triple_inplace_double : forall (p:loc) (n:int),
-  triple (inplace_double p)
-    (p ~~~> n)
-    (fun _ => p ~~~> (2*n)).
+Lemma Triple_inplace_double : forall (p:loc) (n:int),
+  TRIPLE (inplace_double p)
+    PRE (p ~~> n)
+    POST (fun (_:unit) => p ~~> (2*n)).
 Proof using.
-  xwp. xapp. xapp. xapp. xsimpl. math.
+  xwp. xapp. xapp. xapp. xapp. xsimpl. math.
 Qed.
 (* /SOLUTION *)
 
@@ -355,26 +392,26 @@ Definition incr_two : val :=
     incr 'q.
 
 (** The specification of this function takes the form
-    [triple (incr_two p q) H (fun _ => H')],
+    [TRIPLE (incr_two p q) PRE _ POST (fun (r:unit) => _ )],
     where [r] denotes the result value of type unit.
 
-    The precondition describes two references cells: [p ~~~> n]
-    and [q ~~~> m]. To assert that the two cells are distinct from
+    The precondition describes two references cells: [p ~~> n]
+    and [q ~~> m]. To assert that the two cells are distinct from
     each other, we separate their description with the operator [\*].
     This operator called "separating conjunction" in Separation Logic,
     and is also known as the "star" operator. Thus, the precondition
-    is [(p ~~~> n) \* (q ~~~> m)], or simply [p ~~~> n \* q ~~~> m].
+    is [(p ~~> n) \* (q ~~> m)], or simply [p ~~> n \* q ~~> m].
 
     The postcondition describes the final state as
-    is [p ~~~> (n+1) \* q ~~~> (m+1)], where the contents of both
+    is [p ~~> (n+1) \* q ~~> (m+1)], where the contents of both
     cells is increased by one unit compared with the precondition.
 
     The specification triple for [incr_two] is thus as follows. *)
 
-Lemma triple_incr_two : forall (p q:loc) (n m:int),
-  triple (incr_two p q)
-    (p ~~~> n \* q ~~~> m)
-    (fun _ => p ~~~> (n+1) \* q ~~~> (m+1)).
+Lemma Triple_incr_two : forall (p q:loc) (n m:int),
+  TRIPLE (incr_two p q)
+    PRE (p ~~> n \* q ~~> m)
+    POST (fun (r:unit) => p ~~> (n+1) \* q ~~> (m+1)).
 
 (** The verification proof follows the usual pattern. *)
 
@@ -382,25 +419,25 @@ Proof using.
   xwp. xapp. xapp. xsimpl.
 Qed.
 
-(** We register the specification [triple_incr_two] in the
+(** We register the specification [Triple_incr_two] in the
     database, to enable reasoning about calls to [incr_two]. *)
 
-Hint Resolve triple_incr_two : triple.
+Hint Extern 1 (Register_Spec incr_two) => Provide Triple_incr_two.
 
 
 (* ########################################################### *)
 (** ** Aliased arguments *)
 
-(** The specification [triple_incr_two] correctly describes calls to the
+(** The specification [Triple_incr_two] correctly describes calls to the
     function [incr_two] when providing it with two distinct reference cells.
     Yet, it says nothing about a call of the form [incr_two p p].
 
-    Indeed, in Separation Logic, a state described by [p ~~~> n] cannot
-    be matched against a state described by [p ~~~> n \* p ~~~> n], because
+    Indeed, in Separation Logic, a state described by [p ~~> n] cannot
+    be matched against a state described by [p ~~> n \* p ~~> n], because
     the star operator requires its operand to correspond to disjoint pieces
     of state.
 
-    What happens if we nevertheless try to exploit [triple_incr_two]
+    What happens if we nevertheless try to exploit [Triple_incr_two]
     to reason about a call of the form [incr_two p p], that is, with
     aliased arguments?
 
@@ -414,10 +451,10 @@ Definition aliased_call : val :=
 (** A call to [aliased_call p] should increase the contents of [p] by [2].
     This property can be specified as follows. *)
 
-Lemma triple_aliased_call : forall (p:loc) (n:int),
-  triple (aliased_call p)
-    (p ~~~> n)
-    (fun _ => p ~~~> (n+2)).
+Lemma Triple_aliased_call : forall (p:loc) (n:int),
+  TRIPLE (aliased_call p)
+    PRE (p ~~> n)
+    POST (fun (r:unit) => p ~~> (n+2)).
 
 (** If we attempt the proof, we get stuck. Observe how [xapp] reports its
     failure to make progress. *)
@@ -427,46 +464,47 @@ Proof using.
 Abort.
 
 (** In the above proof, we get stuck with a proof obligation of the form:
-    [\[] ==> (p ~~~> ?m) \* _], which requires showing that
-    from an empty state one can extract a reference [p ~~~> ?m]
+    [\[] ==> (p ~~> ?m) \* _], which requires showing that
+    from an empty state one can extract a reference [p ~~> ?m]
     for some integer [?m].
 
-    What happened is that when matching the current state [p ~~~> n]
-    against [p ~~~> ?n \* p ~~~> ?m] (which corresponds to the precondition
-    of [triple_incr_two] with [q = p]), the internal simplification tactic
-    was able to cancel out [p ~~~> n] in both expressions, but then got
-    stuck with matching the empty state against [p ~~~> ?m]. *)
+    What happened is that when matching the current state [p ~~> n]
+    against [p ~~> ?n \* p ~~> ?m] (which corresponds to the precondition
+    of [Triple_incr_two] with [q = p]), the internal simplification tactic
+    was able to cancel out [p ~~> n] in both expressions, but then got
+    stuck with matching the empty state against [p ~~> ?m]. *)
 
-(** The issue here is that the specification [triple_incr_two] is
+(** The issue here is that the specification [Triple_incr_two] is
     specialized for the case of non-aliased references.
 
     It is possible to state and prove an alternative specification for
     the function [incr_two], to cover the case of aliased arguments.
-    Its precondition mentions only one reference, [p ~~~> n], and its
+    Its precondition mentions only one reference, [p ~~> n], and its
     postcondition asserts that its contents gets increased by two units.
 
     This alternative specification can be stated and proved as follows. *)
 
-Lemma triple_incr_two_aliased : forall (p:loc) (n:int),
-  triple (incr_two p p)
-    (p ~~~> n)
-    (fun _ => p ~~~> (n+2)).
+Lemma Triple_incr_two_aliased : forall (p:loc) (n:int),
+  TRIPLE (incr_two p p)
+    PRE (p ~~> n)
+    POST (fun (r:unit) => p ~~> (n+2)).
 Proof using.
   xwp. xapp. xapp. xsimpl. math.
 Qed.
 
 (** By exploiting the alternative specification, we are able to verify
     the specification of [aliased_call p], which invokes [incr_two p p].
-    In order to indicate to the [xapp] tactic that it should invoke the
-    lemma [triple_incr_two_aliased] and not [triple_incr_two], we provide that
-    lemma as argument to [xapp], by writing [xapp triple_incr_two_aliased]. *)
+    In order to indicate to the [xapp] tactic that it should invoke
+    the lemma [Triple_incr_two_aliased] and not [Triple_incr_two],
+    we pass that lemma as argument to [xapp], by writing
+    [xapp Triple_incr_two_aliased]. *)
 
-Lemma triple_aliased_call : forall (p:loc) (n:int),
-  triple (aliased_call p)
-    (p ~~~> n)
-    (fun _ => p ~~~> (n+2)).
+Lemma Triple_aliased_call : forall (p:loc) (n:int),
+  TRIPLE (aliased_call p)
+    PRE (p ~~> n)
+    POST (fun (r:unit) => p ~~> (n+2)).
 Proof using.
-  xwp. xapp triple_incr_two_aliased. xsimpl.
+  xwp. xapp Triple_incr_two_aliased. xsimpl.
 Qed.
 
 
@@ -487,13 +525,13 @@ Definition incr_first : val :=
     incr 'p.
 
 (** We can specify this function by describing its input state
-    as [p ~~~> n \* q ~~~> m], and describing its output state
-    as [p ~~~> (n+1) \* q ~~~> m]. Formally: *)
+    as [p ~~> n \* q ~~> m], and describing its output state
+    as [p ~~> (n+1) \* q ~~> m]. Formally: *)
 
-Lemma triple_incr_first : forall (p q:loc) (n m:int),
-  triple (incr_first p q)
-    (p ~~~> n \* q ~~~> m)
-    (fun _ => p ~~~> (n+1) \* q ~~~> m).
+Lemma Triple_incr_first : forall (p q:loc) (n m:int),
+  TRIPLE (incr_first p q)
+    PRE (p ~~> n \* q ~~> m)
+    POST (fun (r:unit) => p ~~> (n+1) \* q ~~> m).
 Proof using.
   xwp. xapp. xsimpl.
 Qed.
@@ -503,39 +541,39 @@ Qed.
     equally well have described in the specification only the
     existence of the reference that the code manipulates. *)
 
-Lemma triple_incr_first' : forall (p q:loc) (n:int),
-  triple (incr_first p q)
-    (p ~~~> n)
-    (fun _ => p ~~~> (n+1)).
+Lemma Triple_incr_first' : forall (p q:loc) (n:int),
+  TRIPLE (incr_first p q)
+    PRE (p ~~> n)
+    POST (fun (r:unit) => p ~~> (n+1)).
 Proof using.
   xwp. xapp. xsimpl.
 Qed.
 
-(** Interestingly, the specification [triple_incr_first] which
+(** Interestingly, the specification [Triple_incr_first] which
     mentions the two references is derivable from the specification
-    [triple_incr_first'] which mentions only the first reference.
+    [Triple_incr_first'] which mentions only the first reference.
 
     The corresponding proof appears next. It leverages the tactic
     [xtriple], which turns a specification triple of the form
-    [triple t H Q] into the form [PRE H CODE t POST Q], thereby
-    enabling this proof obligation to be processed by [xapp].
+    [TRIPLE _ PRE _ POST _] into the form [PRE _ CODE _ POST _],
+    enabling the proof obligation to be processed by [xapp].
 
-    Here, we invoke the tactic [xapp triple_incr_first'], to
-    exploit the specification [triple_incr_first']. *)
+    Here, we invoke [xapp Triple_incr_first'] to exloit
+    [Triple_incr_first'] for proving [Triple_incr_first]. *)
 
-Lemma triple_incr_first_derived : forall (p q:loc) (n m:int),
-  triple (incr_first p q)
-    (p ~~~> n \* q ~~~> m)
-    (fun _ => p ~~~> (n+1) \* q ~~~> m).
+Lemma Triple_incr_first_derived : forall (p q:loc) (n m:int),
+  TRIPLE (incr_first p q)
+    PRE (p ~~> n \* q ~~> m)
+    POST (fun (r:unit) => p ~~> (n+1) \* q ~~> m).
 Proof using.
-  xtriple. xapp triple_incr_first'. xsimpl.
+  xtriple. xapp Triple_incr_first'. xsimpl.
 Qed.
 
 (** More generally, in Separation Logic, if a specification triple holds,
     then this specification triple remains valid by adding a same heap
-    predicate in both the precondition and the postcondition. This is the
-    "frame" principle, a key modularity feature that we'll come back to
-    later on in the course. *)
+    predicate in both the precondition and the postcondition. This is
+    the "frame" principle, a key modularity feature that we'll come
+    back to later on in the course. *)
 
 
 (* ########################################################### *)
@@ -552,22 +590,19 @@ Qed.
 
 Definition transfer : val :=
   VFun 'p 'q :=
-   Let 'n := '!'p in
-   Let 'm := '!'q in
-   Let 's := 'n '+ 'm in
-   'p ':= 's ';
+   'p ':= ('!'p '+ '!'q) ';
    'q ':= 0.
 
-(* EX1! (triple_transfer) *)
-(** State and prove a lemma called [triple_transfer] specifying
+(* EX1! (Triple_transfer) *)
+(** State and prove a lemma called [Triple_transfer] specifying
     the behavior of [transfer p q] covering the case where [p]
     and [q] denote two distinct references. *)
 
 (* SOLUTION *)
-Lemma triple_transfer : forall (p q:loc) (n m:int),
-  triple (transfer p q)
-    (p ~~~> n \* q ~~~> m)
-    (fun _ => p ~~~> (n + m) \* q ~~~> 0).
+Lemma Triple_transfer : forall (p q:loc) (n m:int),
+  TRIPLE (transfer p q)
+    PRE (p ~~> n \* q ~~> m)
+    POST (fun (_:unit) => p ~~> (n + m) \* q ~~> 0).
 Proof using.
   xwp. xapp. xapp. xapp. xapp. xapp. xsimpl.
 Qed.
@@ -575,16 +610,16 @@ Qed.
 
 (** [] *)
 
-(* EX1! (triple_transfer_aliased) *)
-(** State and prove a lemma called [triple_transfer_aliased] specifying
-    the behavior of [transfer] when it is applied twice to the same
-    argument. It should take the form [triple (transfer p p) H Q]. *)
+(* EX1! (Triple_transfer_aliased) *)
+(** State and prove a lemma called [Triple_transfer_aliased] specifying
+    the behavior of [transfer] when it is applied twice to the same argument.
+    It should take the form [TRIPLE (transfer p p) PRE _ POST _]. *)
 
 (* SOLUTION *)
-Lemma triple_transfer_aliased : forall (p:loc) (n:int),
-  triple (transfer p p)
-    (p ~~~> n)
-    (fun _ => p ~~~> 0).
+Lemma Triple_transfer_aliased : forall (p:loc) (n:int),
+  TRIPLE (transfer p p)
+    PRE (p ~~> n)
+    POST (fun (_:unit) => p ~~> 0).
 Proof using.
   xwp. xapp. xapp. xapp. xapp. xapp. xsimpl.
 Qed.
@@ -594,71 +629,152 @@ Qed.
 
 
 (* ########################################################### *)
+(** *** Existential quantification in heap predicates *)
+
+(** Assume that the programming language includes a built-in
+    random generator function, which expects an integer [n]
+    and outputs an unspecified number between [0] and [n-1]
+    inclusive. *)
+
+Parameter random_int : val.
+
+(** The function [random_int] can be specified as follows.
+
+    Its precondition describes the empty state: [\[]].
+
+    Its postcondition describes an integer [m], whose value
+    is specified to lie in the expected range: [0 <= m < n].
+
+    Formally:
+*)
+
+Parameter Triple_random_int : forall (n:int),
+  TRIPLE (random_int n)
+    PRE \[]
+    POST (fun (m:int) => \[0 <= m < n]).
+
+Hint Extern 1 (Register_Spec random_int) => Provide Triple_random_int.
+
+(** Consider now the following function, which expects an
+    integer [n], and allocates a reference cell whose contents
+    is a random number less than [n].
+
+[[
+    let ref_random_int p =
+      ref (random_int n)
+]]
+*)
+
+Definition ref_random_int : val :=
+  VFun 'n :=
+    'ref (random_int 'n).
+
+(** How can we specify the function [ref_random_int]?
+
+    Its precondition should describe the empty state: [\[]].
+
+    Its postcondition should bind the result value [(p:loc)],
+    which describes the address of the freshly allocated cell.
+    Moreover, it should assert that the memory state is of
+    the form [p ~~> m], for some [m] such that [0 <= m < n].
+
+    We can use the star operator to join the two pieces of
+    information [p ~~> m] and [0 <= m < n] in the postcondition.
+    Doing so, we would obtain:
+
+[[
+    Lemma Triple_ref_random_int : forall (n:int),
+     TRIPLE (ref_random_int n)
+        PRE \[]
+        POST (fun (p:loc) => (p ~~> m) \* \[0 <= m < n]).
+]]
+
+    Yet, this statement does not type-check because [m] is unbound.
+
+    To fix the issue, we need to exploit a new Separation Logic operator:
+    the existential quantifier. Its syntax is [\exists x, _].
+    Observe the use of a leading backslash to distinguish from Coq's
+    standard existential quantifier.
+
+    The correct statement of the specification of [ref_random_int]
+    is thus as follows. *)
+
+Lemma Triple_ref_random_int : forall (n:int),
+  TRIPLE (ref_random_int n)
+    PRE \[]
+    POST (fun (p:loc) => \exists m, (p ~~> m) \* \[0 <= m < n]).
+
+(** Let's comment the proof of this specification step by step. *)
+
+Proof using.
+  xwp.
+  (* We first reason about the call to [random_int@]. *)
+  xapp. intros m Hm.
+  (* Here, [m] denotes the result of [random_int n].
+     This variable is not substituted away because there is no equality
+     of the form [m = _], but instead a constraint [Hm: 0 <= m < n]. *)
+  xapp. intros q.
+  (* Here, [q] denotes the result of [ref m]. *)
+  (* There remains to justify that the current state
+     [q ~~> m] matches the postcondition, which is
+     [\exists m0, q ~~> m0 \* \[0 <= m0 < n]].
+     The simplification tactic [xsimpl] is able to instantiate [m0] as [m]. *)
+  xsimpl.
+  (* There remains to justify the constraint [0 <= m < n].
+     This fact matches exactly the assumption [Hm] obtained earlier. *)
+  auto.
+Qed.
+
+
+(* ########################################################### *)
 (** ** Exercise: allocate a reference with greater contents *)
 
 (** Consider the following function.
 [[
     let ref_greater p =
-      let n = !p in
-      let m = n + 1 in
-      ref m
+      ref (!p + 1)
 ]]
 *)
 
 Definition ref_greater : val :=
   VFun 'p :=
-    Let 'n := '!'p in
-    Let 'm := 'n '+ 1 in
-    'ref 'm.
+    'ref ('!'p '+ 1).
 
-(** The precondition of [ref_greater] asserts the existence of a cell
-    [p ~~~> n]. The postcondition of [ref_greater] asserts the existence
-    of two cells, [p ~~~> n] and [q ~~~> (n+1)], where [q] denotes the
-    location returned by the function.
+(* EX1! (Triple_ref_greater) *)
+(** State a specification for the function [ref_greater], describing
+    precisely the contents of the allocated reference.
 
-    The postcondition of a triple must be of type [val->hprop]. Thus,
-    we need to write the postcondition in the form [fun (r:val) => H'],
-    where [r] denotes the result value, and somehow we need to assert
-    that [r] is a value of the form [val_loc q], for some location [q],
-    where [val_loc] is a coercion from locations to program values.
+    Hint: the postcondition takes the form [POST (fun (q:loc) => _)],
+    where [q] denotes the location of the freshly allocated reference. *)
 
-    To formally relate [r] and [q], we write the postcondition in the
-    form [fun (r:val) => \exists (q:loc), \[r = val_loc q] \* ...].
-    The existential quantifier [\exists] quantifies the variable [q]
-    as part of a heap predicate. The bracket [\[r = val_loc q]] specifies
-    the relation between [r] and [q].
-
-    The complete specification of [ref_greater] is thus as follows. *)
-
-Lemma triple_ref_greater : forall (p:loc) (n:int),
-  triple (ref_greater p)
-    (p ~~~> n)
-    (fun r => \exists q, \[r = val_loc q] \* p ~~~> n \* q ~~~> (n+1)).
+(* SOLUTION *)
+Lemma Triple_ref_greater : forall (p:loc) (n:int),
+  TRIPLE (ref_greater p)
+    PRE (p ~~> n)
+    POST (fun (q:loc) => p ~~> n \* q ~~> (n+1)).
 Proof using.
-  xwp. xapp. xapp. xapp. intros q. xsimpl. auto.
+  xwp. xapp. xapp. xapp. xsimpl.
 Qed.
+(* /SOLUTION *)
 
 (** [] *)
 
-(* EX1! (triple_ref_greater_abstract) *)
+(* EX1! (Triple_ref_greater_abstract) *)
 (** State another specification for the function [ref_greater],
-    called [triple_ref_greater_abstract], with a postcondition that
-    does not reveal the contents of the freshly reference [q], but
-    instead only asserts that its contents is greater than the contents
-    of [p].
+    with a postcondition that does not reveal the contents of
+    the freshly reference [q], but instead only asserts that its
+    contents is greater than the contents of [p].
 
-    Hint: introduce a variable [m] such that [m > n].
-
-    Then, derive the new specification from the former one, following
-    the proof pattern employed in the proof of [triple_incr_first_derived]. *)
+    Then, derive the new specification from the former one, by
+    invoking the tactics [xtriple] and [xapp Triple_ref_greater]. *)
 
 (* SOLUTION *)
-Lemma triple_ref_greater_abstract : forall (p:loc) (n:int),
-  triple (ref_greater p)
-    (p ~~~> n)
-    (fun r => \exists q m, \[r = val_loc q] \* \[m > n] \* q ~~~> m \* p ~~~> n).
+Lemma Triple_ref_greater_abstract : forall (p:loc) (n:int),
+  TRIPLE (ref_greater p)
+    PRE (p ~~> n)
+    POST (fun (q:loc) => \exists m, \[m > n] \* q ~~> m \* p ~~> n).
 Proof using.
-  xtriple. xapp triple_ref_greater. xsimpl. { auto. } { math. }
+  xtriple. xapp Triple_ref_greater. xsimpl. math.
 Qed.
 (* /SOLUTION *)
 
@@ -670,8 +786,8 @@ Qed.
 
 (** Separation Logic tracks allocated data. In its standard setup,
     Separation Logic enforces that all allocated data be eventually
-    deallocated. Technically, the logic is said to "linear" as opposed
-    to "affine". *)
+    deallocated. (Technically, the logic is said to "linear" as opposed
+    to "affine".) *)
 
 (** Let us illustrate what happens when we forget to deallocate data.
     To that end, consider the following program, which computes
@@ -697,35 +813,35 @@ Definition succ_using_incr_attempt :=
     result is [n+1]. Yet, if we try to prove this specification,
     we get stuck. *)
 
-Lemma triple_succ_using_incr_attempt : forall (n:int),
-  triple (succ_using_incr_attempt n)
-    \[]
-    (fun r => \[r = n+1]).
+Lemma Triple_succ_using_incr_attempt : forall (n:int),
+  TRIPLE (succ_using_incr_attempt n)
+    PRE \[]
+    POST (fun r => \[r = n+1]).
 Proof using.
   xwp. xapp. intros p. xapp. xapp. xsimpl. { auto. }
 Abort.
 
 (** In the above proof script, we get stuck with the entailment
-    [p ~~~> (n+1) ==> \[]], which indicates that the current state contains
+    [p ~~> (n+1) ==> \[]], which indicates that the current state contains
     a reference, whereas the postcondition describes an empty state. *)
 
 (** We could attempt to patch the specification to account for the left-over
     reference. This yields a provable specification. *)
 
-Lemma triple_succ_using_incr_attempt' : forall (n:int),
-  triple (succ_using_incr_attempt n)
-    \[]
-    (fun r => \[r = n+1] \* \exists p, (p ~~~> (n+1))).
+Lemma Triple_succ_using_incr_attempt' : forall (n:int),
+  TRIPLE (succ_using_incr_attempt n)
+    PRE \[]
+    POST (fun r => \[r = n+1] \* \exists p, (p ~~> (n+1))).
 Proof using.
   xwp. xapp. intros p. xapp. xapp. xsimpl. { auto. }
 Qed.
 
-(** While the above specification is provable, it is not quite usable.
+(** While the above specification is provable, it is unusable.
 
     Indeed, the above specification features a piece of postcondition
-    [\exists p, p ~~~> (n+1)] that is of absolutely no use to the caller
+    [\exists p, p ~~> (n+1)] that is of absolutely no use to the caller
     of the function. Worse, the caller will have its state polluted with
-    [\exists p, p ~~~> (n+1)] and will have no way to get rid of it apart
+    [\exists p, p ~~> (n+1)] and will have no way to get rid of it apart
     from returning it into its own postcondition. *)
 
 (** The right solution is to patch the code, to free the reference once
@@ -751,30 +867,28 @@ Definition succ_using_incr :=
 
 (** This program may now be proved correct with respect to the intended
     specification. Observe in particular the last call to [xapp] below,
-    which corresponds to the [free] operation.
+    which corresponds to the [free] operation. *)
 
-    The final result is the value of the variable [x]. To reason about it,
-    we exploit the tactic [xval], as illustrated below. *)
-
-Lemma triple_succ_using_incr : forall n,
-  triple (succ_using_incr n)
-    \[]
-    (fun r => \[r = n+1]).
+Lemma Triple_succ_using_incr : forall n,
+  TRIPLE (succ_using_incr n)
+    PRE \[]
+    POST (fun r => \[r = n+1]).
 Proof using.
   xwp. xapp. intros p. xapp. xapp. xapp. xval. xsimpl. auto.
 Qed.
 
-(** Remark: if we verify programs written in a language equipped with
-    a garbage collector (like, e.g., OCaml), we need to tweak the
-    Separation Logic to account for the fact that some heap predicates
-    can be freely discarded from postconditions. This variant of
-    Separation Logic will be described in the chapter [SLFAffine]. *)
+(** Remark: if we verify programs written in a language equipped
+    with a garbage collector (like, e.g., OCaml), we need to
+    tweak the Separation Logic to account for the fact that some
+    heap predicates can be freely discarded from postconditions.
+    This variant of Separation Logic will be described in a bonus
+    chapter ([SLFAffine]). *)
 
 
 (* ########################################################### *)
 (** ** Axiomatization of the mathematical factorial function *)
 
-(** Our next example consists of a program that evaluates the
+(** Our next example consists of a program that evaluate the
     factorial function. To specify this function, we consider
     a Coq axiomatization of the mathematical factorial function,
     which is called [facto]. *)
@@ -796,10 +910,11 @@ Parameter facto_step : forall n,
 (* ########################################################### *)
 (** ** A partial recursive function, without state *)
 
-(** In the rest of the chapter, we will consider recursive functions
-    that manipulate the state. To gently introduce the necessary techniques
-    for reasoning about recursive functions, we first consider a recursive
-    function that does not involve any mutable state.
+(** In the rest of the chapter, we will consider recursive
+    functions that manipulate the state. To gently introduce
+    the necessary technique for reasoning about recursive
+    functions, we first consider a recursive function that does
+    not involve any mutable state.
 
     The function [factorec] computes the factorial of its argument.
 
@@ -808,23 +923,17 @@ Parameter facto_step : forall n,
       if n <= 1 then 1 else n * factorec (n-1)
 ]]
 
-    The corresonding code in A-normal form is slightly more verbose.
 *)
 
 Definition factorec : val :=
   VFix 'f 'n :=
-    Let 'b := 'n '<= 1 in
-    If_ 'b
-      Then 1
-      Else Let 'x := 'n '- 1 in
-           Let 'y := 'f 'x in
-           'n '* 'y.
+    If_ 'n '<= 1 Then 1 Else 'n '* 'f ('n '- 1).
 
 (** A call [factorec n] can be specified as follows:
 
     - the initial state is empty,
     - the final state is empty,
-    - the result value [r] is such that [r = facto n], when [n >= 0].
+    - the result value [r] is such that [r = facto n] when [n >= 0].
 
     In case the argument is negative (i.e., [n < 0]), we have two choices:
 
@@ -845,11 +954,11 @@ Definition factorec : val :=
 
     The specification of [factorec] is thus stated as follows. *)
 
-Lemma triple_factorec : forall n,
+Lemma Triple_factorec : forall n,
   n >= 0 ->
-  triple (factorec n)
-    \[]
-    (fun r => \[r = facto n]).
+  TRIPLE (factorec n)
+    PRE \[]
+    POST (fun (r:int) => \[r = facto n]).
 
 (** We next go through the proof script in details, to explain in particular
     how to set up the induction, how to reason about the recursive call,
@@ -909,14 +1018,14 @@ Proof using.
     xsimpl. rewrite (@facto_step n); math. }
 Qed.
 
-(** Let's revisit the proof script without comments, to get a global
+(** Let's revisit the proof script without comments, to get a better
     picture of the proof structure. *)
 
-Lemma triple_factorec' : forall n,
+Lemma Triple_factorec' : forall n,
   n >= 0 ->
-  triple (factorec n)
-    \[]
-    (fun r => \[r = facto n]).
+  TRIPLE (factorec n)
+    PRE \[]
+    POST (fun (r:int) => \[r = facto n]).
 Proof using.
   intros n. induction_wf IH: (downto 1) n. unfold downto in IH.
   intros Hn. xwp. xapp. xif; intros C.
@@ -929,8 +1038,8 @@ Qed.
 (* ########################################################### *)
 (** ** A recursive function with state *)
 
-(** The example of [factorec] was a warmup. Let's now tackle a recursive
-    function involving some mutable state.
+(** The example of [factorec] was a warmup. Let's now tackle a
+    recursive function involving some mutable state.
 
     The function [repeat_incr p m] makes [m] times a call to [incr p].
     Here, [m] is assumed to be a nonnegative value.
@@ -939,36 +1048,34 @@ Qed.
     let rec repeat_incr p m =
       if m > 0 then (
         incr p;
-        repeat_incr p (m - 1)
+        repeat_incr p (m-1)
       )
 ]]
 *)
 
 Definition repeat_incr : val :=
   VFix 'f 'p 'm :=
-    Let 'b := 'm '> 0 in
-    If_ 'b Then
+    If_ 'm '> 0 Then
       incr 'p ';
-      Let 'x := 'm '- 1 in
-      'f 'p 'x
+      'f 'p ('m '- 1)
     End.
 
 (** The specification for [repeat_incr p] requires that the initial
     state contains a reference [p] with some integer contents [n],
-    that is, [p ~~~> n]. Its postcondition asserts that the resulting
-    state is [p ~~~> (n+m)], which is the result after incrementing
+    that is, [p ~~> n]. Its postcondition asserts that the resulting
+    state is [p ~~> (n+m)], which is the result after incrementing
     [m] times the reference [p]. Observe that this postcondition is
     only valid under the assumption that [m >= 0]. *)
 
-Lemma triple_repeat_incr : forall (m n:int) (p:loc),
+Lemma Triple_repeat_incr : forall (m n:int) (p:loc),
   m >= 0 ->
-  triple (repeat_incr p m)
-    (p ~~~> n)
-    (fun _ => p ~~~> (n + m)).
+  TRIPLE (repeat_incr p m)
+    PRE (p ~~> n)
+    POST (fun (r:unit) => p ~~> (n + m)).
 
-(* EX2! (triple_repeat_incr) *)
-(** Prove the function [triple_repeat_incr].
-    Hint: the structure of the proof resembles that of [triple_factorec']. *)
+(* EX2! (Triple_repeat_incr) *)
+(** Prove the function [Triple_repeat_incr].
+    Hint: the structure of the proof resembles that of [Triple_factorec']. *)
 
 Proof using. (* ADMITTED *)
   intros m. induction_wf IH: (downto 0) m. unfold downto in IH.
@@ -987,11 +1094,11 @@ Qed. (* /ADMITTED *)
     induction. Here is an example illustrating how to deal with such
     a situation. *)
 
-Lemma triple_repeat_incr' : forall (p:loc) (n m:int),
+Lemma Triple_repeat_incr' : forall (p:loc) (n m:int),
   m >= 0 ->
-  triple (repeat_incr p m)
-    (p ~~~> n)
-    (fun _ => p ~~~> (n + m)).
+  TRIPLE (repeat_incr p m)
+    PRE (p ~~> n)
+    POST (fun (r:unit) => p ~~> (n + m)).
 Proof using.
   (* First, introduces all variables and hypotheses. *)
   intros n m Hm.
@@ -1005,7 +1112,7 @@ Abort.
 
 
 (* ########################################################### *)
-(** ** A recursive function involving two references *)
+(** ** Exercise: one-by-one transfer from a reference to another *)
 
 (** Consider the function [step_transfer p q], which repeatedly increment
     a reference [p] and decrement a reference [q], until the contents
@@ -1023,9 +1130,7 @@ Abort.
 
 Definition step_transfer :=
   VFix 'f 'p 'q :=
-    Let 'm := '!'q in
-    Let 'b := 'm '> 0 in
-    If_ 'b Then
+    If_ '! 'q '> 0 Then
       incr 'p ';
       decr 'q ';
       'f 'p 'q
@@ -1036,176 +1141,66 @@ Definition step_transfer :=
     only difference that we here assume the contents of [q] to be
     nonnegative. *)
 
-Lemma triple_step_transfer : forall p q n m,
+Lemma Triple_step_transfer : forall p q n m,
   m >= 0 ->
-  triple (step_transfer p q)
-    (p ~~~> n \* q ~~~> m)
-    (fun _ => p ~~~> (n + m) \* q ~~~> 0).
+  TRIPLE (step_transfer p q)
+    PRE (p ~~> n \* q ~~> m)
+    POST (fun (_:unit) => p ~~> (n + m) \* q ~~> 0).
 
-(* EX2! (triple_step_transfer) *)
+(* EX2! (Triple_step_transfer) *)
 (** Verify the function [step_transfer].
-    Hint: to set up the induction, follow the pattern shown in
-    the proof of [triple_repeat_incr']. *)
+    Hint: to set up the induction, follow the pattern from
+    [Triple_repeat_incr'] presented just above. *)
 
 Proof using. (* ADMITTED *)
   intros q p n m Hm.
   revert n Hm. induction_wf IH: (downto 0) m. unfold downto in IH.
   intros. xwp. xapp. xapp. xif; intros C.
   { xapp. xapp. xapp. { math. } { math. } xsimpl. math. }
-  { xval. xsimpl. { math. } { math. } }
+  { xval. xsimpl. math. math. }
 Qed. (* /ADMITTED *)
 
 (** [] *)
 
 
 (* ########################################################### *)
-(** ** Formalization of the list representation predicate *)
+(* ########################################################### *)
+(* ########################################################### *)
+(** * Optional contents *)
 
-(** A mutable list cell is a two-cell record, featuring a head field and a
-    tail field. We define the field indices as follows. *)
+(* ########################################################### *)
+(** ** Optimized scripts *)
 
-Definition head : field := 0%nat.
-Definition tail : field := 1%nat.
+(** The CFML tool features a number of tricks:
+    - a call to [intros] in front of an [xwp] is always optional,
+    - a single [xapp] in front of an [xif] when the argument
+      of the conditional is a simple boolean test.
 
-(** A mutable list consists of a chain of cells, terminated by [null].
+    Moreover, the TLC library offers a number of useful features:
+    - writing [*] after a tactic name, such as in [xsimpl*],
+      combines the tactic with a call to automation
+      (in short, a combination of [intuition eauto] and [math]),
+    - [unfold downto in IH] is not required because [math] can take care of it,
+    - [introv] is a variant of [intros] that automatically introduces
+      variables, and allows naming only actual hypotheses.
 
-    The heap predicate [MList L p] describes a list whose head cell is
-    at location [p], and whose elements are described by the list [L].
+    Here is an example of a compact proof script for [factorec]. *)
 
-    This predicate is defined recursively on the structure of [L]:
-
-    - if [L] is empty, then [p] is the null pointer,
-    - if [L] is of the form [x::L'], then the head field of [p]
-      contains [x], and the tail field of [p] contains a pointer
-      [q] such that [MList L' q] describes the tail of the list.
-
-*)
-
-Fixpoint MList (L:list val) (p:loc) : hprop :=
-  match L with
-  | nil => \[p = null]
-  | x::L' => \exists q, (p`.head ~~> x) \* (p`.tail ~~> q)
-                     \* (MList L' q)
-  end.
-
-(** The following reformulations of the definition are helpful in proofs,
-    allowing to fold or unfold the definition using a tactic called
-    [xchange]. *)
-
-Lemma MList_nil : forall p,
-  (p ~> MList nil) = \[p = null].
-Proof using. auto. Qed.
-
-Lemma MList_cons : forall p x L',
-  p ~> MList (x::L') =
-  \exists q, (p`.head ~~> x) \* (p`.tail ~~> q) \* MList L' q.
-Proof using.  auto. Qed.
-
-(** Another characterization of [MList L p] is useful for proofs. Whereas
-    the original definition is by case analysis on whether [L] is empty,
-    the alternative one is by case analysis on whether [p] is null:
-
-    - if [p] is null, then [L] is empty,
-    - otherwise, [L] decomposes as [x::L'], the head field of [p] contains [x],
-      and the tail field of [p] contains a pointer [q] such that [MList L' q]
-      describes the tail of the list.
-
-    The lemma below is stated using an entailment. The reciprocal entailment
-    is also true, but we do not need it so we do not bother proving it here.
-*)
-
-Lemma MList_if : forall (p:loc) (L:list val),
-      (MList L p)
-  ==> (If p = null
-      then \[L = nil]
-      else \exists x q L', \[L = x::L']
-           \* (p`.head ~~> x) \* (p`.tail ~~> q)
-           \* (MList L' q)).
+Lemma Triple_factorec'' : forall n,
+  n >= 0 ->
+  TRIPLE (factorec n)
+    PRE \[]
+    POST (fun (r:int) => \[r = facto n]).
 Proof using.
-  (* Let's prove this result by case analysis on [L]. *)
-  intros. destruct L as [|x L'].
-  { (* Case [L = nil]. By definition of [MList], we have [p = null]. *)
-    xchange MList_nil. intros M.
-    (* We have to justify [L = nil], which is trivial.
-       The TLC [case_if] tactic performs a case analysis on the argument
-       of the first visible [if] conditional. *)
-    case_if. xsimpl. auto. }
-  { (* Case [L = x::L']. *)
-  (* One possibility is to perform a rewrite operation using [MList_cons]
-     on its first occurrence. Then using CFML the tactic [xpull] to extract
-     the existential quantifiers out from the precondition:
-     [rewrite MList_cons. xpull. intros q.]
-     A more efficient approach is to use the dedicated CFML tactic [xchange],
-     which is specialized for performing updates in the current state. *)
-    xchange MList_cons. intros q. case_if.
-    { (* Case [p = null]. Contradiction because nothing can be allocated at
-         the null location, as captured by lemma [Hfield_not_null],
-         which states: [(l`.f ~~> V) ==> (l`.f ~~> V) \* \[l <> null]]. *)
-      subst. lets: hfield_not_null. xchange hfield_not_null. }
-    { (* Case [p <> null]. The 'else' branch corresponds to the definition
-         of [MList] in the [cons] case. It suffices to correctly instantiate
-         the existential quantifiers. *)
-      xsimpl. auto. } }
+  introv Hn. gen Hn. induction_wf IH: (downto 1) n.
+  xwp. xif; intros C.
+  { xval. xsimpl. rewrite* facto_init. }
+  { xapp. xapp*. xapp. xsimpl. rewrite* (@facto_step n). }
 Qed.
 
 
 (* ########################################################### *)
-(** ** In-place concatenation of two mutable lists *)
-
-(** The following function expects a nonempty list [p1] and a list [p2],
-    and updates [p1] in place so that its tail gets extended by the
-    cells from [p2].
-
-[[
-    let rec append p1 p2 =
-      if p1.tail == null
-        then p1.tail <- p2
-        else append p1.tail p2
-]]
-
-*)
-
-Definition append : val :=
-  VFix 'f 'p1 'p2 :=
-    Let 'q1 := 'p1'.tail in
-    Let 'b := ('q1 '= null) in
-    If_ 'b
-      Then Set 'p1'.tail ':= 'p2
-      Else 'f 'q1 'p2.
-
-(** The append function is specified and verified as follows. *)
-
-Lemma Triple_append : forall (L1 L2:list val) (p1 p2:loc),
-  p1 <> null ->
-  triple (append p1 p2)
-    (MList L1 p1 \* MList L2 p2)
-    (fun _ => MList (L1++L2) p1).
-Proof using.
-  (* The induction principle provides an hypothesis for the tail of [L1],
-      i.e., for the list [L1'] such that the relation [list_sub L1' L1] holds. *)
-  introv K. gen p1. induction_wf IH: (@list_sub val) L1. introv N. xwp.
-  (* To begin the proof, we reveal the head cell of [p1].
-     We let [q1] denote the tail of [p1], and [L1'] the tail of [L1]. *)
-  xchange (MList_if p1). case_if. xpull. intros x q1 L1' ->.
-  (* We then reason about the case analysis. *)
-  xapp. xapp. xif; intros Cq1.
-  { (* If [q1'] is null, then [L1'] is empty. *)
-    xchange (MList_if q1). case_if. xpull. intros ->.
-    (* In this case, we set the pointer, then we fold back the head cell. *)
-    xapp. xchange <- MList_cons. }
-  { (* If [q1'] is not null, we reason about the recursive call using
-       the induction hypothesis, then we fold back the head cell. *)
-    xapp. xchange <- MList_cons. }
-Qed.
-
-
-(* ########################################################### *)
-(* ########################################################### *)
-(* ########################################################### *)
-(** * Bonus contents (optional reading) *)
-
-(* ########################################################### *)
-(** ** Trying to prove incorrect specifications (optional) *)
+(** ** Trying to prove incorrect specifications *)
 
 (** Recall the function [repeat_incr p n], which invokes [n]
     times [incr p].
@@ -1214,7 +1209,7 @@ Qed.
     let rec repeat_incr p m =
       if m > 0 then (
         incr p;
-        repeat_incr p (m - 1)
+        repeat_incr p (m-1)
       )
 ]]
 *)
@@ -1224,13 +1219,13 @@ Qed.
 
     Clearly, something should break in the proof, because when [m < 0],
     the call [repeat_incr p m] terminates immediately. Thus, when [m < 0]
-    the final state is like the initial state [p ~~~> n], and not equal
-    to [p ~~~> (n + m)]. Let us investigate how the proof breaks. *)
+    the final state is like the initial state [p ~~> n], and not equal
+    to [p ~~> (n + m)]. Let us investigate how the proof breaks. *)
 
-Lemma triple_repeat_incr_incorrect : forall (p:loc) (n m:int),
-  triple (repeat_incr p m)
-    (p ~~~> n)
-    (fun _ => p ~~~> (n + m)).
+Lemma Triple_repeat_incr_incorrect : forall (p:loc) (n m:int),
+  TRIPLE (repeat_incr p m)
+    PRE (p ~~> n)
+    POST (fun (_:unit) => p ~~> (n + m)).
 Proof using.
   intros. revert n. induction_wf IH: (downto 0) m. unfold downto in IH.
   intros. xwp. xapp. xif; intros C.
@@ -1239,7 +1234,7 @@ Proof using.
   { (* In the 'else' branch: [m <= 0] *)
     xval.
     (* Here, we are requested to justify that the current state
-       [p ~~~> n] matches the postcondition [p ~~~> (n + m)], which
+       [p ~~> n] matches the postcondition [p ~~> (n + m)], which
        amounts to proving [n = n + m]. *)
     xsimpl.
     (* When the specification features the assumption [m >= 0],
@@ -1251,12 +1246,12 @@ Abort.
 
 (** Note that there exists a valid specification for [repeat_incr] that
     does not constraint [m], but instead specifies that the state
-    always evolves from [p ~~~> n] to [p ~~~> (n + max 0 m)]. *)
+    always evolves from [p ~~> n] to [p ~~> (n + max 0 m)]. *)
 
-Lemma triple_repeat_incr' : forall (p:loc) (n m:int),
-  triple (repeat_incr p m)
-    (p ~~~> n)
-    (fun _ => p ~~~> (n + max 0 m)).
+Lemma Triple_repeat_incr' : forall (p:loc) (n m:int),
+  TRIPLE (repeat_incr p m)
+    PRE (p ~~> n)
+    POST (fun (_:unit) => p ~~> (n + max 0 m)).
 
 (** Let's prove the above specification, which, by the way, is the
     most-general specification for the function [repeat_incr].
@@ -1272,9 +1267,43 @@ Lemma triple_repeat_incr' : forall (p:loc) (n m:int),
 *)
 
 Proof using.
-  intros. gen n. induction_wf IH: (downto 0) m.
+  intros. gen n. induction_wf IH: (downto 0) m. unfold downto.
   xwp. xapp. xif; intros C.
-  { xapp. xapp. xapp. { math. }  
+  { xapp. xapp. xapp. { math. }
     xsimpl. repeat rewrite max_r; math. }
   { xval. xsimpl. rewrite max_l; math. }
 Qed.
+
+
+(* ########################################################### *)
+(** ** Incorrect quantification of existential variables *)
+
+(** Recall the function [ref_random_int n], defined as
+    [ref (random_int n)].
+
+    Consider the following specification, which quantifies [m]
+    outside of the triple, rather than using a [\exists] in the
+    postcondition. *)
+
+Parameter Triple_ref_random_int_incorrect : forall (n:int) (m:int),
+  TRIPLE (ref_random_int n)
+    PRE \[]
+    POST (fun (p:loc) => (p ~~> m) \* \[0 <= m < n]).
+
+(* QUIZ *)
+
+(** What does this specification mean? It is useful? Is it provable? *)
+
+(* /QUIZ *)
+
+(** Answer: no function can admit this specification, because it
+    could be instantiated, say, with [m=0] to prove that the output
+    reference contains the integer [0]; and also with [m=1] to prove
+    that the output reference contains the integer [1]; the two
+    instantiations contradict each other. *)
+
+(** As a general rule, variables that are not arguments of the function,
+    nor variables used in the preconditions (i.e., "ghost arguments"),
+    should be bound in the postcondition, either as the return value
+    (like [fun (p:loc) => _], or using a Separation Logic existential
+    quantifier (e.g., [\exists m, _]). *)
